src/program_proof/session/versionVector.v
@@ -1,0 +1,2 @@
+Require Import Perennial.program_proof.session.session_definitions.
+Import ServerSide SessionServer.
